src/Init/Data/Vector.lean
@@ -10,4 +10,5 @@ import Init.Data.Vector.Lex
 import Init.Data.Vector.MapIdx
 import Init.Data.Vector.Count
 import Init.Data.Vector.DecidableEq
+import Init.Data.Vector.Zip
 import Init.Data.Vector.OfFn
